platform/Safety.v
@@ -1,0 +1,80 @@
+Require Import Bedrock PreAutoSep Sys.
+Import XCAP.
+
+
+Section OpSem.
+  Variable m : module.
+  Variable stn : settings.
+  Variable prog : program.
+
+  Hypothesis inj : forall l1 l2 w, Labels stn l1 = Some w
+    -> Labels stn l2 = Some w
+    -> l1 = l2.
+
+  Hypothesis agree : forall l pre bl, LabelMap.MapsTo l (pre, bl) (Blocks m)
+    -> exists w, Labels stn l = Some w
+      /\ prog w = Some bl.
+
+  Hypothesis agreeImp : forall l pre, LabelMap.MapsTo l pre (Imports m)
+    -> exists w, Labels stn l = Some w
+      /\ prog w = None
+      /\ l = ("sys", Global "abort")
+      /\ pre = Precondition abortS None.
+
+  Hypothesis omitImp : forall l w,
+    Labels stn ("sys", l) = Some w
+    -> prog w = None.
+
+  Hypothesis ok : moduleOk m.
+
+  Hint Constructors reachable sys_step.
+
+  Lemma reachable_sys : forall st st',
+    sys_reachable stn prog st st'
+    -> reachable stn prog st st'
+    \/ (reachable stn prog st st'
+      /\ Labels stn ("sys", Global "abort") = Some (fst st')).
+    induction 1; intuition.
+
+    destruct H; eauto.
+
+    destruct H; eauto.
+  Qed.
+
+  Lemma safe_sys : forall st,
+    safe stn prog st
+    -> sys_safe stn prog st.
+    unfold sys_safe; post.
+    apply reachable_sys in H0; post.
+
+    specialize (H _ H1).
+    case_eq (step stn prog st'); intuition eauto.
+
+    specialize (H _ H0).
+    unfold step in H.
+    apply omitImp in H2.
+    rewrite H2 in *.
+    tauto.
+  Qed.
+
+  Theorem safety : forall st l pre bl, LabelMap.MapsTo l (pre, bl) (Blocks m)
+    -> Labels stn l = Some (fst st)
+    -> interp (specs0 m stn) (pre (stn, snd st))
+    -> sys_safe stn prog st.
+    intros; hnf; intros.
+
+    apply reachable_sys in H2; post.
+
+    eapply safety'' in H3; eauto.
+    post.
+    apply agreeImp in H4; post; subst.
+    eauto.
+    case_eq (step stn prog st'); intros; eauto; congruence.
+    
+    intros.
+    apply agreeImp in H2.
+    post; eauto.
+
+    eauto.
+  Qed.
+End OpSem.
